BinaryHeap.lean
@@ -54,11 +54,11 @@ def indexOf {α : Type u} {le : α → α → Bool} {n : Nat} : BinaryHeap α le
 
 instance : GetElem (BinaryHeap α le n) (Nat) α (λ _ index ↦ index > 0 ∧ index < n) where
   getElem := λ heap index h₁ ↦ match n, heap, index with
-  | (_+1), {tree, ..}, index => tree.get ⟨index, h₁.right⟩
+  | (_+1), {tree, ..}, index => tree.get' ⟨index, h₁.right⟩
 
 instance : GetElem (BinaryHeap α le n) (Fin n) α (λ _ _ ↦ n > 0) where
   getElem := λ heap index _ ↦ match n, heap, index with
-  | (_+1), {tree, ..}, index => tree.get index
+  | (_+1), {tree, ..}, index => tree.get' index
 
 /--Helper for the common case of using natural numbers for sorting.-/
 theorem nat_ble_to_heap_le_total : total_le Nat.ble := by
