BinaryHeap/CompleteTree/AdditionalProofs.lean
@@ -2,17 +2,153 @@ import BinaryHeap.CompleteTree.Lemmas
 import BinaryHeap.CompleteTree.AdditionalOperations
 import BinaryHeap.CompleteTree.HeapOperations
 
-namespace BinaryHeap
+namespace BinaryHeap.CompleteTree.AdditionalProofs
+
+private theorem if_get_eq_contains {α : Type u} {o : Nat} (tree : CompleteTree α (o+1)) (element : α) (index : Fin (o+1)) : tree.get' index = element → tree.contains element := by
+    unfold get' contains
+    simp only [Nat.succ_eq_add_one, Fin.zero_eta, Nat.add_eq, ne_eq]
+    split
+    case h_1 p q v l r _ _ _ _ =>
+      intro h₁
+      split; omega
+      rename α => vv
+      rename_i hsum heq
+      have h₂ := heqSameRoot (hsum) (Nat.succ_pos (p+q)) heq
+      rw[root_unfold] at h₂
+      rw[root_unfold] at h₂
+      simp only [←h₂, h₁, true_or]
+    case h_2 index p q v l r _ _ _ _ h₃ =>
+      intro h₄
+      split ; rename_i hx _; exact absurd hx (Nat.succ_ne_zero _)
+      case h_2 pp qq vv ll rr _ _  _ h₅ heq =>
+      have : p = pp := heqSameLeftLen h₅ (Nat.succ_pos _) heq
+      have : q = qq := heqSameRightLen h₅ (Nat.succ_pos _) heq
+      subst pp qq
+      simp only [Nat.add_eq, Nat.succ_eq_add_one, heq_eq_eq, branch.injEq] at heq
+      have : v = vv := heq.left
+      have : l = ll := heq.right.left
+      have : r = rr := heq.right.right
+      subst vv ll rr
+      revert h₄
+      split
+      all_goals
+        split
+        intro h₄
+        right
+      case' isTrue => left
+      case' isFalse => right
+      all_goals
+        revert h₄
+        apply if_get_eq_contains
+        done
+
+private theorem if_contains_get_eq_auxl {α : Type u} {o : Nat} (tree : CompleteTree α (o+1)) (element : α) (h₁ : o > 0) :
+  have : tree.leftLen (Nat.lt_succ_of_lt h₁) > 0 := by
+    unfold leftLen;
+    split
+    unfold length
+    rename_i hx _ _
+    simp only [Nat.add_eq, Nat.succ_eq_add_one, Nat.reduceEqDiff] at hx
+    omega
+  ∀(indexl : Fin (tree.leftLen (Nat.succ_pos o))), (tree.left _).get indexl this = element → ∃(index : Fin (o+1)), tree.get index (Nat.lt_succ_of_lt h₁) = element
+:= by
+  simp
+  intro indexl
+  let index : Fin (o+1) := indexl.succ.castLT (by
+    simp only [Nat.succ_eq_add_one, Fin.val_succ, Nat.succ_lt_succ_iff, gt_iff_lt]
+    exact Nat.lt_of_lt_of_le indexl.isLt $ Nat.le_of_lt_succ $ leftLenLtN tree (Nat.succ_pos o)
+  )
+  intro prereq
+  exists index
+  unfold get
+  simp
+  unfold get'
+  generalize hindex : index = i
+  split
+  case h_1 =>
+    have : index.val = 0 := Fin.val_eq_of_eq hindex
+    contradiction
+  case h_2 j p q v l r ht1 ht2 ht3 _ _ =>
+    have h₂ : index.val = indexl.val + 1 := rfl
+    have h₃ : index.val = j.succ := Fin.val_eq_of_eq hindex
+    have h₄ : j = indexl.val := Nat.succ.inj $ h₃.subst (motive := λx↦ x = indexl.val + 1) h₂
+    have : p = (branch v l r ht1 ht2 ht3).leftLen (Nat.succ_pos _) := rfl
+    have h₅ : j < p := by simp only [this, indexl.isLt, h₄]
+    simp only [h₅, ↓reduceDite, Nat.add_eq]
+    unfold get at prereq
+    split at prereq
+    rename_i pp ii ll _ hel hei heq _
+    split
+    rename_i ppp lll _ _ _ _ _ _ _
+    have : pp = ppp := by omega
+    subst pp
+    simp only [gt_iff_lt, Nat.succ_eq_add_one, Nat.add_eq, heq_eq_eq, Nat.zero_lt_succ] at *
+    have : j = ii.val := by omega
+    subst j
+    simp
+    rw[←hei] at prereq
+    rw[left_unfold] at heq
+    rw[heq]
+    assumption
+
+private theorem if_contains_get_eq {α : Type u} {o : Nat} (tree : CompleteTree α (o+1)) (element : α) (h₁ : tree.contains element) : ∃(index : Fin (o+1)), tree.get' index = element := by
+    revert h₁
+    unfold contains
+    split ; rename_i hx _; exact absurd hx (Nat.succ_ne_zero o)
+    rename_i n m v l r _ _ _ he heq
+    intro h₁
+    cases h₁
+    case h_2.inl h₂ =>
+      unfold get'
+      exists 0
+      split
+      case h_2 hx => have hx := Fin.val_eq_of_eq hx; simp at hx;
+      case h_1 vv _ _ _ _ _ _ _ =>
+        have h₃ := heqSameRoot he (Nat.succ_pos _) heq
+        simp only[root_unfold] at h₃
+        simp only[h₃, h₂]
+    rename_i h
+    cases h
+    case h_2.inr.inl h₂ => exact
+      match hn : n, hl: l with
+      | 0, .leaf => by contradiction
+      | (nn+1), l => by
+        have nn_lt_o : nn < o := by have : o = nn + 1 + m := Nat.succ.inj he; omega
+        have blah := if_contains_get_eq l element h₂
+        have blupp := if_contains_get_eq_auxl tree element $ Nat.zero_lt_of_lt nn_lt_o
+        simp at blupp
+        simp[get_eq_get'] at blah ⊢
+        apply blah.elim
+        match o, tree with
+        | (yy+_), .branch _ ll _ _ _ _ =>
+          simp_all[left_unfold, leftLen_unfold]
+          have : yy = nn+1 := heqSameLeftLen (by omega) (Nat.succ_pos _) heq
+          subst yy
+          have : _ = m := heqSameRightLen (by omega) (Nat.succ_pos _) heq
+          subst m
+          simp_all
+          exact blupp
+    case h_2.inr.inr h₂ => sorry
+  termination_by o
+
+
+theorem contains_iff_index_exists {α : Type u} {o : Nat} (tree : CompleteTree α (o+1)) (element : α) : tree.contains element ↔ ∃ (index : Fin (o+1)), tree.get' index = element := by
+  constructor
+  case mpr =>
+    simp only [forall_exists_index]
+    exact if_get_eq_contains tree element
+  case mp =>
+    exact if_contains_get_eq tree element
 
 /--Shows that the index and value returned by heapRemoveLastWithIndex are consistent.-/
-private theorem CompleteTree.heapRemoveLastWithIndexReturnsItemAtIndex {α : Type u} {o : Nat} (heap : CompleteTree α (o+1)) : heap.get heap.heapRemoveLastWithIndex.snd.snd = heap.heapRemoveLastWithIndex.snd.fst := by
+protected theorem heapRemoveLastWithIndexReturnsItemAtIndex {α : Type u} {o : Nat} (heap : CompleteTree α (o+1)) : heap.get' heap.heapRemoveLastWithIndex.snd.snd = heap.heapRemoveLastWithIndex.snd.fst := by
   unfold CompleteTree.heapRemoveLastWithIndex CompleteTree.Internal.heapRemoveLastAux
   split
   rename_i n m v l r m_le_n max_height_difference subtree_full
   simp only [Nat.add_eq, Fin.zero_eta, Fin.isValue, decide_eq_true_eq, Fin.castLE_succ]
   split
   case isTrue n_m_zero =>
-    unfold get
+    unfold get'
     split
     case h_1 nn mm vv ll rr mm_le_nn _ _ _ _ he₁ he₂ =>
       have h₁ : n = 0 := And.left $ Nat.add_eq_zero.mp n_m_zero.symm
@@ -24,7 +160,7 @@ private theorem CompleteTree.heapRemoveLastWithIndexReturnsItemAtIndex {α : Typ
     case h_2 =>
       omega -- to annoying to deal with Fin.ofNat... There's a hypothesis that says 0 = ⟨1,_⟩.
   case isFalse n_m_not_zero =>
-    unfold get
+    unfold get'
     split
     case h_1 nn mm vv ll rr mm_le_nn max_height_difference_2 subtree_full2 _ he₁ he₂ he₃ =>
       --aaaaaaaaaaaaaaaaaaaaaaaaaaaaaa
@@ -81,5 +217,5 @@ private theorem CompleteTree.heapRemoveLastWithIndexReturnsItemAtIndex {α : Typ
         simp only [this, ↓reduceDite, Nat.pred_succ, Fin.isValue]
         subst j -- overkill, but unlike rw it works
         simp only [Nat.pred_succ, Fin.isValue, Nat.add_sub_cancel, Fin.eta]
-        apply heapRemoveLastWithIndexReturnsItemAtIndex
+        apply AdditionalProofs.heapRemoveLastWithIndexReturnsItemAtIndex
         done
