BinaryHeap/CompleteTree/Lemmas.lean
@@ -1,4 +1,5 @@
 import BinaryHeap.CompleteTree.Basic
+import BinaryHeap.CompleteTree.AdditionalOperations
 import BinaryHeap.HeapPredicate
 
 namespace BinaryHeap
@@ -21,17 +22,31 @@ theorem CompleteTree.root_unfold {α : Type u} {o p : Nat} (v : α) (l : Complet
 /-- Helper to rw away left, because Lean 4.9 makes it unnecessarily hard to deal with match in tactics mode... -/
 theorem CompleteTree.left_unfold {α : Type u} {o p : Nat} (v : α) (l : CompleteTree α o) (r : CompleteTree α p) (h₁ : p ≤ o) (h₂ : o < 2 * (p + 1)) (h₃ : (o + 1).isPowerOfTwo ∨ (p + 1).isPowerOfTwo) (h₄ : o + p + 1 > 0): (CompleteTree.branch v l r h₁ h₂ h₃).left h₄ = l := rfl
 
+theorem CompleteTree.leftLen_unfold {α : Type u} {o p : Nat} (v : α) (l : CompleteTree α o) (r : CompleteTree α p) (h₁ : p ≤ o) (h₂ : o < 2 * (p + 1)) (h₃ : (o + 1).isPowerOfTwo ∨ (p + 1).isPowerOfTwo) (h₄ : o + p + 1 > 0): (CompleteTree.branch v l r h₁ h₂ h₃).leftLen h₄ = o := rfl
+
 /-- Helper to rw away right, because Lean 4.9 makes it unnecessarily hard to deal with match in tactics mode... -/
 theorem CompleteTree.right_unfold {α : Type u} {o p : Nat} (v : α) (l : CompleteTree α o) (r : CompleteTree α p) (h₁ : p ≤ o) (h₂ : o < 2 * (p + 1)) (h₃ : (o + 1).isPowerOfTwo ∨ (p + 1).isPowerOfTwo) (h₄ : o + p + 1 > 0): (CompleteTree.branch v l r h₁ h₂ h₃).right h₄ = r := rfl
 
 theorem CompleteTree.heqSameLeftLen {α : Type u} {n m : Nat} {a : CompleteTree α n} {b : CompleteTree α m} (h₁ : n = m) (h₂ : n > 0) (h₃ : HEq a b) : a.leftLen h₂ = b.leftLen (h₁.subst h₂) := by
   subst n
   have h₃ : a = b := eq_of_heq h₃
-  subst a
-  rfl
+  congr
 
 theorem CompleteTree.heqSameRightLen {α : Type u} {n m : Nat} {a : CompleteTree α n} {b : CompleteTree α m} (h₁ : n = m) (h₂ : n > 0) (h₃ : HEq a b) : a.rightLen h₂ = b.rightLen (h₁.subst h₂) := by
   subst n
   have h₃ : a = b := eq_of_heq h₃
-  subst a
-  rfl
+  congr
+
+theorem CompleteTree.heqSameRoot {α : Type u} {n m : Nat} {a : CompleteTree α n} {b : CompleteTree α m} (h₁ : n = m) (h₂ : n > 0) (h₃ : HEq a b) : a.root h₂ = b.root (h₁.subst h₂) := by
+  subst n
+  have h₃ : a = b := eq_of_heq h₃
+  congr
+
+theorem CompleteTree.get_eq_get' {α : Type u} {n : Nat} (tree : CompleteTree α (n+1)) (index : Fin (n+1)) : tree.get' index = tree.get index (Nat.succ_pos n) := rfl
+
+theorem CompleteTree.leftLenLtN {α : Type u} {n : Nat} (tree : CompleteTree α n) (h₁ : n>0) : tree.leftLen h₁ < n := by
+  unfold leftLen
+  split
+  rw[length]
+  rename_i o p _ _ _ _ _ _ _
+  exact Nat.lt_of_le_of_lt (Nat.le_add_right o p) (Nat.lt_succ_self (o+p))
